examples/new_stack/NewStack23Aproof.v
@@ -1,0 +1,221 @@
+Require Import NewStack2 NewStack3A HoareDef SimModSem.
+Require Import Coqlib.
+Require Import Universe.
+Require Import Skeleton.
+Require Import PCM.
+Require Import ModSem Behavior.
+Require Import Relation_Definitions.
+
+(*** TODO: export these in Coqlib or Universe ***)
+Require Import Relation_Operators.
+Require Import RelationPairs.
+From ITree Require Import
+     Events.MapDefault.
+From ExtLib Require Import
+     Core.RelDec
+     Structures.Maps
+     Data.Map.FMapAList.
+Require Import TODOYJ.
+Require Import HTactics Logic IPM.
+Require Import OpenDef.
+Require Import TODO.
+
+Set Implicit Arguments.
+
+Local Open Scope nat_scope.
+
+
+
+Section SIMMODSEM.
+
+  Context `{Σ: GRA.t}.
+  Context `{@GRA.inG stkRA Σ}.
+
+  Let W: Type := ((Σ * Any.t)) * ((Σ * Any.t)).
+
+(*   Let wf: W -> Prop := *)
+(*     @mk_wf _ unit *)
+(*            (fun _ _ _stk_mgr0 => *)
+(*               (∃ (stk_mgr0: gmap mblock (list Z)), *)
+(*                   (⌜<<CAST: _stk_mgr0 = stk_mgr0↑>>⌝) ∧ *)
+(*                   (OwnM (Auth.black ([∗ map] handle ↦ stk ∈ stk_mgr0, *)
+(*                                      (_is_stack handle stk)))) *)
+(*               )%I) *)
+(*            (fun _ _ _ => ⌜True⌝%I) *)
+(*   . *)
+(*   (big_opM bi_sep (fun k x => P) m) *)
+(* ([∗ map] handle ↦ stk ∈ stk_mgr0, *)
+(*                              (∃ hd, OwnM ((handle, 0%Z) |-> [hd]) ** is_list hd (map Vint stk))) *)
+  Let wf: W -> Prop :=
+    @mk_wf _ unit
+           (fun _ _ _stk_mgr0 =>
+              (∃ (stk_mgr0: gmap mblock (list Z)) (stk_res0: URA.car (t:=_stkRA)),
+                  (⌜(<<PHYS: _stk_mgr0 = stk_mgr0↑>>) /\
+                   (<<SIM: forall h stk, stk_res0 h = Some stk <-> stk_mgr0 !! h = Some stk>>)⌝)
+                  ∧ (OwnM ((Auth.black stk_res0): URA.car (t:=stkRA)))
+              )%I)
+           (fun _ _ _ => ⌜True⌝%I)
+  .
+
+  (* Lemma is_stack_nil *)
+  (*       h *)
+  (*   : *)
+  (*     (is_stack h []) = ε *)
+  (* . *)
+  (* Proof. *)
+  (*   unfold is_stack. ss. unfold Auth.white. f_equal. unfold _is_stack. extensionality _h. des_ifs. ss. *)
+  (* Qed. *)
+
+
+
+  Section AUX.
+    Context {K: Type} `{M: URA.t}.
+    Let RA := URA.pointwise K M.
+
+    Lemma pw_extends (f0 f1: K -> M) (EXT: @URA.extends RA f0 f1): <<EXT: forall k, URA.extends (f0 k) (f1 k)>>.
+    Proof. ii. r in EXT. des. subst. ur. ss. eexists; et. Qed.
+    (* Lemma pw_unfold_wf (f: K -> M): (forall k, URA.wf (f k)) -> @URA.wf RA f. Proof. i. ss. Qed. *)
+
+    (* Lemma empty_wf: forall k, URA.wf ((@URA.unit RA) k). *)
+    (* Proof. ii; ss. eapply URA.wf_unit. Qed. *)
+
+    (* Lemma update_wf: forall `{Dec K} (f: @URA.car RA) k v (WF: URA.wf f) (WF: URA.wf v), URA.wf (update f k v: (@URA.car RA)). *)
+    (* Proof. ii. unfold update. des_ifs; ss. Qed. *)
+
+    Lemma pw_wf: forall (f: @URA.car RA) (WF: URA.wf f), <<WF: forall k, URA.wf (f k)>>.
+    Proof. ii; ss. rewrite URA.unfold_wf in WF. ss. Qed.
+
+  End AUX.
+
+  Theorem sim_modsem: ModSemPair.sim (NewStack3A.StackSem) (NewStack2.StackSem).
+  Proof.
+    econstructor 1 with (wf:=wf); ss; et; swap 2 3.
+    { econs; ss.
+      - eapply to_semantic; cycle 1. { admit "ez - wf". } iIntros "H". iExists _, _. iSplit; ss; et.
+      - eapply to_semantic; cycle 1. { eapply URA.wf_unit. } iIntros "H". iPureIntro. ss.
+    }
+    econs; ss.
+    { unfold NewStack2.new_body, cfun. init. harg. fold wf. mDesAll. des; clarify.
+      apply Any.upcast_inj in PURE0. des; clarify. steps. rewrite Any.upcast_downcast in *. clarify. steps.
+      astart 0. astop. steps. rewrite Any.upcast_downcast in *. clarify.
+      rename g into stk_mgr0. rename x0 into h. rename a1 into stk_res0. force_l. exists (Vptr h 0). steps.
+      mOwnWf "A".
+      assert(WF1: forall k, stk_res0 k <> Excl.boom).
+      { eapply Auth.black_wf in WF0. eapply pw_wf in WF0. des. ii. specialize (WF0 k). rewrite H0 in WF0.
+        ur in WF0. ss. }
+
+      hret _; ss.
+      { iPoseProof (OwnM_Upd with "A") as "A".
+        { eapply Auth.auth_alloc2. instantiate (1:=(_is_stack h [])).
+          ur. i. specialize (WF1 k).
+          destruct (dec k h).
+          - subst. ur.
+            destruct (stk_res0 h) eqn:T; ss.
+            + erewrite SIM in T. clarify.
+            + unfold _is_stack. des_ifs.
+          - ur.
+            destruct (stk_res0 k) eqn:T; ss.
+            + unfold _is_stack. des_ifs.
+            + unfold _is_stack. des_ifs.
+        }
+        iMod "A". iDestruct "A" as "[A B]". iModIntro. iSplitL "A"; et.
+        iExists _, _. iSplit; ss; et. iSplit; ss; et. iPureIntro. ii.
+        assert(B: stk_res0 h = Excl.unit).
+        { destruct (stk_res0 h) eqn:T; ss.
+          - rewrite SIM in T. rewrite T in *. ss.
+          - exploit WF1; et; ss.
+        }
+        clear - SIM WF1 B.
+        destruct (dec h h0).
+        - subst. rewrite lookup_insert.
+          ur. ur. unfold _is_stack. des_ifs_safe. ss. clarify. split; i; clarify.
+        - rewrite lookup_insert_ne; ss.
+          ur. ur. unfold _is_stack. des_ifs_safe. ss. erewrite <- SIM. split; i; des_ifs.
+      }
+    }
+    econs; ss.
+    { unfold NewStack2.pop_body, cfun. init. harg. fold wf. des_ifs_safe. mDesAll. des; clarify.
+      apply Any.upcast_inj in PURE0. des; clarify. steps. rewrite Any.upcast_downcast in *. clarify. steps.
+      astart 0. astop. steps. rewrite Any.upcast_downcast in *. clarify.
+      rename g into stk_mgr0. rename n into h. rename a1 into stk_res0.
+      mCombine "A1" "A".
+      mOwnWf "A1".
+      assert(A: forall k, URA.wf ((stk_res0 k): URA.car (t:=Excl.t _))).
+      { eapply URA.wf_mon in WF0.
+        eapply Auth.black_wf in WF0. eapply pw_wf in WF0. des. ii. specialize (WF0 k). ss. }
+      assert(B: stk_res0 h = Some l).
+      { dup WF0.
+        eapply Auth.auth_included in WF0. des. unfold _is_stack in WF0. eapply pw_extends in WF0. des.
+        spc WF0. des_ifs. ss. eapply Excl.extends in WF0; ss. }
+      assert(C:=B). eapply SIM in C. rewrite C. steps.
+      destruct l as [|x stk].
+      - steps. force_l. esplits. steps. hret _; ss.
+        iDestruct "A1" as "[A B]".
+        iModIntro. iFrame. iSplit; ss; et.
+      - steps. Auth.auth_update
+      force_l. exists (Vptr h 0). steps.
+      mOwnWf "A".
+      assert(WF1: forall k, stk_res0 k <> Excl.boom).
+      { ur in WF0. des. r in WF1. repeat ur in WF1. rewrite Seal.sealing_eq in WF1. hexploit (WF1); et. }
+
+      hret _; ss.
+      { iPoseProof (OwnM_Upd with "A") as "A".
+        { eapply Auth.auth_alloc2. instantiate (1:=(_is_stack h [])).
+          ur. i. specialize (WF1 k).
+          destruct (dec k h).
+          - subst. ur.
+            destruct (stk_res0 h) eqn:T; ss.
+            + erewrite SIM in T. clarify.
+            + unfold _is_stack. des_ifs.
+          - ur.
+            destruct (stk_res0 k) eqn:T; ss.
+            + unfold _is_stack. des_ifs.
+            + unfold _is_stack. des_ifs.
+        }
+        iMod "A". iDestruct "A" as "[A B]". iModIntro. iSplitL "A"; et.
+        iExists _, _. iSplit; ss; et. iSplit; ss; et. iPureIntro. ii.
+        assert(B: stk_res0 h = Excl.unit).
+        { destruct (stk_res0 h) eqn:T; ss.
+          - rewrite SIM in T. rewrite T in *. ss.
+          - exploit WF1; et; ss.
+        }
+        clear - SIM WF1 B.
+        destruct (dec h h0).
+        - subst. rewrite lookup_insert.
+          ur. ur. unfold _is_stack. des_ifs_safe. ss. clarify. split; i; clarify.
+        - rewrite lookup_insert_ne; ss.
+          ur. ur. unfold _is_stack. des_ifs_safe. ss. erewrite <- SIM. split; i; des_ifs.
+      }
+    }
+
+    split; i.
+
+          spc SIM. specialize (SIM []).
+          rewrite <- SIM. lookup rewrite fn_lookup_insert. ss.
+          ur.
+          { iPureIntro.
+      }
+      admit "mid - somehow".
+    }
+    admit "mid - somehow".
+  Unshelve.
+    all: ss.
+  Qed.
+
+End SIMMODSEM.
+
+
+
+Section SIMMOD.
+
+  Context `{Σ: GRA.t}.
+  Context `{@GRA.inG memRA Σ}.
+
+  Theorem correct: ModPair.sim (NewStack2.Stack) (KMod.to_src NewStack1.KStack).
+  Proof.
+    econs; ss.
+    { ii. eapply adequacy_lift. eapply sim_modsem; ss. }
+    ii; ss. repeat (Psimpl; econs; ss).
+  Qed.
+
+End SIMMOD.
